utp/utp_subst.thy
@@ -472,16 +472,16 @@ subsection {* Conditional Substitution Laws *}
   
 lemma usubst_cond_upd_1 [usubst]:
   "\<sigma>(x \<mapsto>\<^sub>s u) \<triangleleft> b \<triangleright>\<^sub>s \<rho>(x \<mapsto>\<^sub>s v) = (\<sigma> \<triangleleft> b \<triangleright>\<^sub>s \<rho>)(x \<mapsto>\<^sub>s u \<triangleleft> b \<triangleright> v)"
-  by (simp add: cond_subst_def subst_upd_uvar_def, transfer, auto)
+  by (simp add: cond_subst_def subst_upd_uvar_def uexpr_defs, transfer, auto)
 
 lemma usubst_cond_upd_2 [usubst]:
   "\<lbrakk> vwb_lens x; x \<sharp> \<rho> \<rbrakk> \<Longrightarrow> \<sigma>(x \<mapsto>\<^sub>s u) \<triangleleft> b \<triangleright>\<^sub>s \<rho> = (\<sigma> \<triangleleft> b \<triangleright>\<^sub>s \<rho>)(x \<mapsto>\<^sub>s u \<triangleleft> b \<triangleright> &x)"
-  by (simp add: cond_subst_def subst_upd_uvar_def unrest_usubst_def, transfer)
+  by (simp add: cond_subst_def subst_upd_uvar_def unrest_usubst_def uexpr_defs, transfer)
      (metis (full_types, hide_lams) id_apply pr_var_def subst_upd_uvar_def usubst_upd_pr_var_id var.rep_eq)
  
 lemma usubst_cond_upd_3 [usubst]:
   "\<lbrakk> vwb_lens x; x \<sharp> \<sigma> \<rbrakk> \<Longrightarrow> \<sigma> \<triangleleft> b \<triangleright>\<^sub>s \<rho>(x \<mapsto>\<^sub>s v) = (\<sigma> \<triangleleft> b \<triangleright>\<^sub>s \<rho>)(x \<mapsto>\<^sub>s &x \<triangleleft> b \<triangleright> v)"
-  by (simp add: cond_subst_def subst_upd_uvar_def unrest_usubst_def, transfer)
+  by (simp add: cond_subst_def subst_upd_uvar_def unrest_usubst_def uexpr_defs, transfer)
      (metis (full_types, hide_lams) id_apply pr_var_def subst_upd_uvar_def usubst_upd_pr_var_id var.rep_eq)
     
 lemma usubst_cond_id [usubst]:
